backend/Deadcodeproof.v
@@ -24,6 +24,7 @@ Require Import Memory.
 Require Import Globalenvs.
 Require Import Events.
 Require Import Smallstep.
+Require Import Language.
 Require Import Op.
 Require Import Registers.
 Require Import RTL.
@@ -34,6 +35,8 @@ Require Import ValueAnalysis.
 Require Import NeedDomain.
 Require Import NeedOp.
 Require Import Deadcode.
+Require Import Linkeq.
+Require Import SepcompRel.
 
 (** * Relating the memory states *)
 
@@ -366,63 +369,75 @@ Qed.
 
 Section PRESERVATION.
 
+Let transf_efT (p:program) (ef:external_function) := OK ef.
+
 Variable prog: program.
 Variable tprog: program.
-Hypothesis TRANSF: transf_program prog = OK tprog.
+Hypothesis TRANSF:
+  @sepcomp_rel
+    Language_RTL Language_RTL
+    (fun p f tf => transf_function (romem_for_program p) f = OK tf)
+    (fun p ef tef => transf_efT p ef = OK tef)
+    (@OK _)
+    prog tprog.
 Let ge := Genv.globalenv prog.
 Let tge := Genv.globalenv tprog.
-Let rm := romem_for_program prog.
 
 Lemma symbols_preserved:
   forall (s: ident), Genv.find_symbol tge s = Genv.find_symbol ge s.
-Proof.
-  intro. unfold ge, tge.
-  apply Genv.find_symbol_transf_partial with (transf_fundef rm).
-  exact TRANSF.
-Qed.
+Proof (find_symbol_transf_partial _ _ TRANSF).
 
 Lemma varinfo_preserved:
   forall b, Genv.find_var_info tge b = Genv.find_var_info ge b.
-Proof.
-  intro. unfold ge, tge.
-  apply Genv.find_var_info_transf_partial with (transf_fundef rm).
-  exact TRANSF.
-Qed.
+Proof (find_var_info_transf_partial _ _ TRANSF).
 
 Lemma functions_translated:
   forall (v: val) (f: RTL.fundef),
   Genv.find_funct ge v = Some f ->
-  exists tf,
-  Genv.find_funct tge v = Some tf /\ transf_fundef rm f = OK tf.
-Proof (Genv.find_funct_transf_partial (transf_fundef rm) _ TRANSF).
+  exists tf, Genv.find_funct tge v = Some tf /\ 
+             exists sprog, program_linkeq Language_RTL sprog prog /\
+                           transf_fundef (romem_for_program sprog) f = OK tf.
+Proof.
+  intros. exploit (find_funct_transf_partial _ _ TRANSF); eauto. simpl in *.
+  intros [tf [Htf [sprog [Hsprog Hf]]]].
+  eexists. split; eauto. eexists. split; eauto.
+  destruct f; monadInv Hf; auto.
+  unfold transf_fundef. unfold transf_partial_fundef.
+  rewrite EQ. auto.
+Qed.
 
 Lemma function_ptr_translated:
   forall (b: block) (f: RTL.fundef),
   Genv.find_funct_ptr ge b = Some f ->
-  exists tf,
-  Genv.find_funct_ptr tge b = Some tf /\ transf_fundef rm f = OK tf.
-Proof (Genv.find_funct_ptr_transf_partial (transf_fundef rm) _ TRANSF).
+  exists tf, Genv.find_funct_ptr tge b = Some tf /\ 
+             exists sprog, program_linkeq Language_RTL sprog prog /\
+                           transf_fundef (romem_for_program sprog) f = OK tf.
+Proof.
+  intros. exploit (find_funct_ptr_transf_partial _ _ TRANSF); eauto. simpl in *.
+  intros [tf [Htf [sprog [Hsprog Hf]]]].
+  eexists. split; eauto. eexists. split; eauto.
+  destruct f; monadInv Hf; auto.
+  unfold transf_fundef. unfold transf_partial_fundef.
+  rewrite EQ. auto.
+Qed.
 
 Lemma sig_function_translated:
-  forall f tf,
-  transf_fundef rm f = OK tf ->
-  funsig tf = funsig f.
+  forall sprog f tf, transf_fundef (romem_for_program sprog) f = OK tf -> funsig tf = funsig f.
 Proof.
-  intros; destruct f; monadInv H.
+  unfold transf_fundef; intros. destruct f; monadInv H; auto.
   unfold transf_function in EQ. 
-  destruct (analyze (vanalyze rm f) f); inv EQ; auto. 
-  auto.
+  destruct (analyze (vanalyze (romem_for_program sprog) f) f); try discriminate. inv EQ; auto. 
 Qed.
 
 Lemma stacksize_translated:
-  forall f tf,
+  forall rm f tf,
   transf_function rm f = OK tf -> tf.(fn_stacksize) = f.(fn_stacksize).
 Proof.
   unfold transf_function; intros. destruct (analyze (vanalyze rm f) f); inv H; auto.
 Qed.
 
 Lemma transf_function_at:
-  forall f tf an pc instr,
+  forall rm f tf an pc instr,
   transf_function rm f = OK tf ->
   analyze (vanalyze rm f) f = Some an ->
   f.(fn_code)!pc = Some instr ->
@@ -457,7 +472,10 @@ Lemma find_function_translated:
   forall ros rs fd trs ne,
   find_function ge ros rs = Some fd ->
   eagree rs trs (add_ros_need_all ros ne) ->
-  exists tfd, find_function tge ros trs = Some tfd /\ transf_fundef rm fd = OK tfd.
+  exists tfd, find_function tge ros trs = Some tfd /\ 
+              exists sprog,
+                program_linkeq Language_RTL sprog prog /\
+                transf_fundef (romem_for_program sprog) fd = OK tfd.
 Proof.
   intros. destruct ros as [r|id]; simpl in *.
 - assert (LD: Val.lessdef rs#r trs#r) by eauto with na. inv LD.
@@ -471,30 +489,33 @@ Qed.
 
 Inductive match_stackframes: stackframe -> stackframe -> Prop :=
   | match_stackframes_intro:
-      forall res f sp pc e tf te an
-        (FUN: transf_function rm f = OK tf)
-        (ANL: analyze (vanalyze rm f) f = Some an)
+      forall res f sp pc e tf te an sprog
+        (FUN: transf_function (romem_for_program sprog) f = OK tf)
+        (ANL: analyze (vanalyze (romem_for_program sprog) f) f = Some an)
+        (SPROG: program_linkeq Language_RTL sprog prog)
         (RES: forall v tv,
               Val.lessdef v tv ->
               eagree (e#res <- v) (te#res<- tv)
-                     (fst (transfer f (vanalyze rm f) pc an!!pc))),
+                     (fst (transfer f (vanalyze (romem_for_program sprog) f) pc an!!pc))),
       match_stackframes (Stackframe res f (Vptr sp Int.zero) pc e)
                         (Stackframe res tf (Vptr sp Int.zero) pc te).
 
 Inductive match_states: state -> state -> Prop :=
   | match_regular_states:
-      forall s f sp pc e m ts tf te tm an
+      forall s f sp pc e m ts tf te tm an sprog
         (STACKS: list_forall2 match_stackframes s ts)
-        (FUN: transf_function rm f = OK tf)
-        (ANL: analyze (vanalyze rm f) f = Some an)
-        (ENV: eagree e te (fst (transfer f (vanalyze rm f) pc an!!pc)))
-        (MEM: magree m tm (nlive ge sp (snd (transfer f (vanalyze rm f) pc an!!pc)))),
+        (FUN: transf_function (romem_for_program sprog) f = OK tf)
+        (ANL: analyze (vanalyze (romem_for_program sprog) f) f = Some an)
+        (SPROG: program_linkeq Language_RTL sprog prog)
+        (ENV: eagree e te (fst (transfer f (vanalyze (romem_for_program sprog) f) pc an!!pc)))
+        (MEM: magree m tm (nlive ge sp (snd (transfer f (vanalyze (romem_for_program sprog) f) pc an!!pc)))),
       match_states (State s f (Vptr sp Int.zero) pc e m)
                    (State ts tf (Vptr sp Int.zero) pc te tm)
   | match_call_states:
-      forall s f args m ts tf targs tm
+      forall s f args m ts tf targs tm sprog
         (STACKS: list_forall2 match_stackframes s ts)
-        (FUN: transf_fundef rm f = OK tf)
+        (FUN: transf_fundef (romem_for_program sprog) f = OK tf)
+        (SPROG: program_linkeq Language_RTL sprog prog)
         (ARGS: Val.lessdef_list args targs)
         (MEM: Mem.extends m tm),
       match_states (Callstate s f args m)
@@ -510,7 +531,7 @@ Inductive match_states: state -> state -> Prop :=
 (** [match_states] and CFG successors *)
 
 Lemma analyze_successors:
-  forall f an pc instr pc',
+  forall rm f an pc instr pc',
   analyze (vanalyze rm f) f = Some an ->
   f.(fn_code)!pc = Some instr ->
   In pc' (successors_instr instr) ->
@@ -521,10 +542,11 @@ Proof.
 Qed.
 
 Lemma match_succ_states:
-  forall s f sp pc e m ts tf te tm an pc' instr ne nm
+  forall s f sp pc e m ts tf te tm an pc' instr ne nm sprog
     (STACKS: list_forall2 match_stackframes s ts)
-    (FUN: transf_function rm f = OK tf)
-    (ANL: analyze (vanalyze rm f) f = Some an)
+    (FUN: transf_function (romem_for_program sprog) f = OK tf)
+    (ANL: analyze (vanalyze (romem_for_program sprog) f) f = Some an)
+    (SPROG: program_linkeq Language_RTL sprog prog)
     (INSTR: f.(fn_code)!pc = Some instr)
     (SUCC: In pc' (successors_instr instr))
     (ANPC: an!!pc = (ne, nm))
@@ -605,7 +627,7 @@ Qed.
 
 Theorem step_simulation:
   forall S1 t S2, step ge S1 t S2 ->
-  forall S1', match_states S1 S1' -> sound_state prog S1 ->
+  forall S1', match_states S1 S1' -> sound_state_ext prog S1 ->
   exists S2', step tge S1' t S2' /\ match_states S2 S2'.
 Proof.
 
@@ -614,7 +636,7 @@ Ltac TransfInstr :=
   | [INSTR: (fn_code _)!_ = Some _,
      FUN: transf_function _ _ = OK _,
      ANL: analyze _ _ = Some _ |- _ ] =>
-       generalize (transf_function_at _ _ _ _ _ FUN ANL INSTR);
+       generalize (transf_function_at _ _ _ _ _ _ FUN ANL INSTR);
        intro TI;
        unfold transf_instr in TI
   end.
@@ -719,7 +741,7 @@ Ltac UseTransfer :=
 
 - (* store *)
   TransfInstr; UseTransfer.
-  destruct (nmem_contains nm (aaddressing (vanalyze rm f) # pc addr args)
+  destruct (nmem_contains nm (aaddressing (vanalyze (romem_for_program sprog) f) # pc addr args)
              (size_chunk chunk)) eqn:CONTAINS.
 + (* preserved *)
   simpl in *. 
@@ -748,10 +770,10 @@ Ltac UseTransfer :=
 
 - (* call *)
   TransfInstr; UseTransfer.
-  exploit find_function_translated; eauto 2 with na. intros (tfd & A & B).
+  exploit find_function_translated; eauto 2 with na. intros (tfd & A & sprog' & Hsprog' & B).
   econstructor; split.
-  eapply exec_Icall; eauto. apply sig_function_translated; auto. 
-  constructor. 
+  eapply exec_Icall; eauto. eapply sig_function_translated; eauto. 
+  econstructor; eauto. 
   constructor; auto. econstructor; eauto. 
   intros.
   edestruct analyze_successors; eauto. simpl; eauto. 
@@ -761,18 +783,18 @@ Ltac UseTransfer :=
 
 - (* tailcall *)
   TransfInstr; UseTransfer.
-  exploit find_function_translated; eauto 2 with na. intros (tfd & A & B).
+  exploit find_function_translated; eauto 2 with na. intros (tfd & A & sprog' & Hsprog' & B).
   exploit magree_free. eauto. eauto. instantiate (1 := nlive ge stk nmem_all). 
   intros; eapply nlive_dead_stack; eauto. 
   intros (tm' & C & D). 
   econstructor; split.
-  eapply exec_Itailcall; eauto. apply sig_function_translated; auto. 
+  eapply exec_Itailcall; eauto. eapply sig_function_translated; eauto. 
   erewrite stacksize_translated by eauto. eexact C.
-  constructor; eauto 2 with na. eapply magree_extends; eauto. apply nlive_all.
+  econstructor; eauto 2 with na. eapply magree_extends; eauto. apply nlive_all.
 
 - (* builtin *)
   TransfInstr; UseTransfer. revert ENV MEM TI. 
-  functional induction (transfer_builtin (vanalyze rm f)#pc ef args res ne nm);
+  functional induction (transfer_builtin (vanalyze (romem_for_program sprog) f)#pc ef args res ne nm);
   simpl in *; intros.
 + (* volatile load *)
   assert (LD: Val.lessdef rs#a1 te#a1) by eauto 2 with na.
@@ -803,7 +825,7 @@ Ltac UseTransfer :=
     inv H2. 
   * exists (Val.load_result chunk v0); split; auto. constructor; auto. 
   * exploit magree_load; eauto.
-    inv SS. intros. eapply nlive_add; eauto. constructor. apply GE. auto. 
+    inv SS. specialize (Hsound _ SPROG). inv Hsound. intros. eapply nlive_add; eauto. constructor. apply GE. auto. 
     intros (tv & P & Q). 
     exists tv; split; auto. constructor; auto. 
   }
@@ -844,10 +866,10 @@ Ltac UseTransfer :=
 + (* memcpy *)
   rewrite e1 in TI.
   inv H0. 
-  set (adst := aaddr (vanalyze rm f) # pc dst) in *.
-  set (asrc := aaddr (vanalyze rm f) # pc src) in *.
+  set (adst := aaddr (vanalyze (romem_for_program sprog) f) # pc dst) in *.
+  set (asrc := aaddr (vanalyze (romem_for_program sprog) f) # pc src) in *.
   exploit magree_loadbytes. eauto. eauto. 
-  exploit aaddr_sound. eauto. symmetry; eexact H2.
+  exploit aaddr_sound; eauto. 
   intros (bc & A & B & C).
   intros. eapply nlive_add; eassumption. 
   intros (tbytes & P & Q).
@@ -857,7 +879,7 @@ Ltac UseTransfer :=
   intros. apply incl_nmem_add; auto.
   eauto. 
   instantiate (1 := nlive ge sp0 nm). 
-  exploit aaddr_sound. eauto. symmetry; eexact H1.
+  exploit aaddr_sound. eauto. eauto. symmetry; eexact H1.
   intros (bc & A & B & C).
   intros. eapply nlive_remove; eauto.
   erewrite Mem.loadbytes_length in H10 by eauto. 
@@ -875,14 +897,14 @@ Ltac UseTransfer :=
   apply eagree_update; eauto 3 with na.
 + (* memcpy eliminated *)
   rewrite e1 in TI. inv H0.
-  set (adst := aaddr (vanalyze rm f) # pc dst) in *.
-  set (asrc := aaddr (vanalyze rm f) # pc src) in *.
+  set (adst := aaddr (vanalyze (romem_for_program sprog) f) # pc dst) in *.
+  set (asrc := aaddr (vanalyze (romem_for_program sprog) f) # pc src) in *.
   econstructor; split.
   eapply exec_Inop; eauto. 
   eapply match_succ_states; eauto. simpl; auto.
   apply eagree_set_undef; auto.
   eapply magree_storebytes_left; eauto.
-  exploit aaddr_sound. eauto. symmetry; eexact H1.
+  exploit aaddr_sound. eauto. eauto. symmetry; eexact H1.
   intros (bc & A & B & C).
   intros. eapply nlive_contains; eauto.
   erewrite Mem.loadbytes_length in H0 by eauto. 
@@ -953,7 +975,7 @@ Ltac UseTransfer :=
 
 - (* internal function *)
   monadInv FUN. generalize EQ. unfold transf_function. intros EQ'.
-  destruct (analyze (vanalyze rm f) f) as [an|] eqn:AN; inv EQ'.
+  destruct (analyze (vanalyze (romem_for_program sprog) f) f) as [an|] eqn:AN; inv EQ'.
   exploit Mem.alloc_extends; eauto. apply Zle_refl. apply Zle_refl.
   intros (tm' & A & B). 
   econstructor; split.
@@ -984,14 +1006,15 @@ Lemma transf_initial_states:
   exists st2, initial_state tprog st2 /\ match_states st1 st2.
 Proof.
   intros. inversion H.
-  exploit function_ptr_translated; eauto. intros (tf & A & B).
+  exploit function_ptr_translated; eauto. intros (tf & A & sprog & Hsprog & B).
   exists (Callstate nil tf nil m0); split.
   econstructor; eauto.
-  eapply Genv.init_mem_transf_partial; eauto.
-  rewrite (transform_partial_program_main _ _ TRANSF).
+  exploit (init_mem_transf_partial _ _ TRANSF); eauto.
+  replace (prog_main tprog) with (prog_main prog).
   rewrite symbols_preserved. eauto.
-  rewrite <- H3. apply sig_function_translated; auto.
-  constructor. constructor. auto. constructor. apply Mem.extends_refl.
+  inv TRANSF. auto.
+  rewrite <- H3. eapply sig_function_translated; eauto.
+  econstructor; eauto. constructor. apply Mem.extends_refl.
 Qed.
 
 Lemma transf_final_states:
@@ -1008,17 +1031,32 @@ Theorem transf_program_correct:
 Proof.
   intros.
   apply forward_simulation_step with
-     (match_states := fun s1 s2 => sound_state prog s1 /\ match_states s1 s2).
+     (match_states := fun s1 s2 => sound_state_ext prog s1 /\ match_states s1 s2).
 - exact symbols_preserved.
 - simpl; intros. exploit transf_initial_states; eauto. intros [st2 [A B]].
   exists st2; intuition. eapply sound_initial; eauto. 
 - simpl; intros. destruct H. eapply transf_final_states; eauto. 
 - simpl; intros. destruct H0.
-  assert (sound_state prog s1') by (eapply sound_step; eauto).
+  assert (sound_state_ext prog s1') by (eapply sound_past_step; eauto).
   fold ge; fold tge. exploit step_simulation; eauto. intros [st2' [A B]].
   exists st2'; auto. 
 Qed.
 
 End PRESERVATION.
 
-
+Lemma Deadcode_sepcomp_rel
+      rtlprog1 rtlprog2
+      (Htrans: Deadcode.transf_program rtlprog1 = OK rtlprog2):
+  @sepcomp_rel
+    Language.Language_RTL Language.Language_RTL
+    (fun p f tf => Deadcode.transf_function (ValueAnalysis.romem_for_program p) f = OK tf)
+    (fun p ef tef => (fun _ ef => OK ef) p ef = OK tef)
+    (@OK _)
+    rtlprog1 rtlprog2.
+Proof.
+  apply transf_partial_sepcomp_rel.
+  unfold progT, RTL.program, RTL.fundef in *. simpl in *. rewrite <- Htrans.
+  unfold Deadcode.transf_program. f_equal.
+  apply Axioms.functional_extensionality. intro fd.
+  destruct fd; auto.
+Qed.
