backend/Selectionproof.v
@@ -22,6 +22,7 @@ Require Import Memory.
 Require Import Events.
 Require Import Globalenvs.
 Require Import Smallstep.
+Require Import Language.
 Require Import Switch.
 Require Import Cminor.
 Require Import Op.
@@ -33,10 +34,15 @@ Require Import Selection.
 Require Import SelectOpproof.
 Require Import SelectDivproof.
 Require Import SelectLongproof.
+Require Import MapsExtra.
+Require Import Linker.
+Require Import LinkerProp.
+Require Import Linkeq.
+Require Import SepcompRel.
+Require Import CoqlibExtra.
 
 Local Open Scope cminorsel_scope.
 Local Open Scope error_monad_scope.
-
 
 (** * Correctness of the instruction selection functions for expressions *)
 
@@ -48,41 +54,83 @@ Let ge := Genv.globalenv prog.
 Let tge := Genv.globalenv tprog.
 Hypothesis HELPERS:
   forall name sg, In (name, sg) i64_helpers -> helper_declared ge name sg.
-Hypothesis TRANSFPROG: transform_partial_program (sel_fundef ge) prog = OK tprog.
+Hypothesis TRANSF:
+  @sepcomp_rel
+    Language_Cminor Language_CminorSel
+    (fun p f tf =>
+       sel_function (Genv.globalenv p) f = OK tf)
+    (fun p ef tef =>
+       ef = tef)
+    (@OK _)
+    prog tprog.
+
+Let prog_match:
+  match_program
+    (fun fd tfd =>
+       exists sprog, program_linkeq Language_Cminor sprog prog /\
+       sel_fundef (Genv.globalenv sprog) fd = OK tfd)
+    (fun info tinfo => info = tinfo)
+    nil prog.(prog_main)
+    prog tprog.
+Proof.
+  destruct prog as [defs ?], tprog as [tdefs ?]. clear HELPERS.
+  inv TRANSF. simpl in *. subst. clear ge tge.
+  revert tdefs Hdefs. generalize defs at 1 3 as fdefs.
+  induction defs; intros fdefs tdefs Hdefs.
+  { inv Hdefs. constructor; auto. exists nil. split; auto. constructor. }
+  inv Hdefs. destruct a, b1, H1 as [? H1]. simpl in *. subst.
+  eapply IHdefs in H3. destruct H3 as [H3 ?]. split; [|auto].
+  destruct H3 as [? H3]. simpl in *. rewrite app_nil_r in *.
+  destruct H3 as [H3 ?]. subst.
+  eexists. rewrite app_nil_r. split; auto.
+  constructor; auto.
+  destruct H1 as [prog_src [Hprog_src H1]]. inv H1.
+  - apply match_glob_fun. eexists. split; eauto.
+    simpl in *. destruct fd_src; inv Hf_src. destruct fd_tgt; inv Hf_tgt.
+    unfold sel_fundef, transf_partial_fundef. rewrite Hf. auto.
+  - apply match_glob_fun. eexists. split; eauto.
+    simpl in *. destruct fd_src; inv Hef_src. destruct fd_tgt; inv Hef_tgt.
+    unfold sel_fundef, transf_partial_fundef. auto.
+  - unfold transf_globvar in Hv. monadInv Hv. inv EQ.
+    destruct gv_src. constructor. auto.
+Qed.
 
 Lemma symbols_preserved:
   forall (s: ident), Genv.find_symbol tge s = Genv.find_symbol ge s.
 Proof.
-  intros. eapply Genv.find_symbol_transf_partial; eauto. 
+  intros. eapply Genv.find_symbol_match; eauto.
 Qed.
 
 Lemma function_ptr_translated:
   forall (b: block) (f: Cminor.fundef),
   Genv.find_funct_ptr ge b = Some f ->
-  exists tf, Genv.find_funct_ptr tge b = Some tf /\ sel_fundef ge f = OK tf.
-Proof.  
-  intros. eapply Genv.find_funct_ptr_transf_partial; eauto.
-Qed.
+  exists tf, Genv.find_funct_ptr tge b = Some tf /\
+  exists sprog, program_linkeq Language_Cminor sprog prog /\
+  sel_fundef (Genv.globalenv sprog) f = OK tf.
+Proof. intros. exploit Genv.find_funct_ptr_match; eauto. Qed.
 
 Lemma functions_translated:
   forall (v v': val) (f: Cminor.fundef),
   Genv.find_funct ge v = Some f ->
   Val.lessdef v v' ->
-  exists tf, Genv.find_funct tge v' = Some tf /\ sel_fundef ge f = OK tf.
-Proof.  
-  intros. inv H0.
-  eapply Genv.find_funct_transf_partial; eauto.
-  simpl in H. discriminate.
+  exists tf, Genv.find_funct tge v' = Some tf /\
+  exists sprog, program_linkeq Language_Cminor sprog prog /\
+  sel_fundef (Genv.globalenv sprog) f = OK tf.
+Proof.
+  intros. exploit Genv.find_funct_match; eauto.
+  intros [tf [Htf [sprog [Hsprog hf]]]].
+  eexists; split; eauto.
+  inv H0; auto. inv H.
 Qed.
 
 Lemma sig_function_translated:
-  forall f tf, sel_fundef ge f = OK tf -> funsig tf = Cminor.funsig f.
+  forall ge f tf, sel_fundef ge f = OK tf -> funsig tf = Cminor.funsig f.
 Proof.
   intros. destruct f; monadInv H; auto. monadInv EQ. auto. 
 Qed.
 
 Lemma stackspace_function_translated:
-  forall f tf, sel_function ge f = OK tf -> fn_stackspace tf = Cminor.fn_stackspace f.
+  forall ge f tf, sel_function ge f = OK tf -> fn_stackspace tf = Cminor.fn_stackspace f.
 Proof.
   intros. monadInv H. auto. 
 Qed.
@@ -90,7 +138,12 @@ Qed.
 Lemma varinfo_preserved:
   forall b, Genv.find_var_info tge b = Genv.find_var_info ge b.
 Proof.
-  intros; eapply Genv.find_var_info_transf_partial; eauto.
+  intros. destruct (Genv.find_var_info ge b) as [v|] eqn:V.
+  - exploit Genv.find_var_info_match; eauto. intros [tv [A B]]. inv B. assumption.
+  - destruct (Genv.find_var_info tge b) as [v'|] eqn:V'; auto.
+    exploit Genv.find_var_info_rev_match; eauto.
+    simpl. destruct (plt b (Genv.genv_next (Genv.globalenv prog))); try tauto.
+    intros [v [A B]]. inv B. fold ge in A. congruence.
 Qed.
 
 Lemma helper_declared_preserved:
@@ -98,6 +151,7 @@ Lemma helper_declared_preserved:
 Proof.
   intros id sg (b & A & B).
   exploit function_ptr_translated; eauto. simpl. intros (tf & P & Q). inv Q. 
+  inv H. inv H1.
   exists b; split; auto. rewrite symbols_preserved. auto.
 Qed.
 
@@ -269,6 +323,63 @@ Proof.
   predSpec Int.eq Int.eq_spec i0 Int.zero; congruence.
 Qed.
 
+Lemma find_symbol_spec (p:Cminor.program) i:
+  match Genv.find_symbol (Genv.globalenv p) i, option_map snd (find (fun id => peq i (fst id)) (rev p.(prog_defs))) with
+    | Some b, Some g =>
+      match
+        g,
+        Genv.find_funct_ptr (Genv.globalenv p) b,
+        Genv.find_var_info (Genv.globalenv p) b
+      with
+        | Gfun fd1, Some fd2, None => fd1 = fd2
+        | Gvar vi1, None, Some vi2 => vi1 = vi2
+        | _, _, _ => False
+      end
+    | None, None => True
+    | _, _ => False
+  end.
+Proof.
+  Ltac clarify :=
+    repeat (try match goal with
+                  | [H1: ?m ! ?b = _, H2: ?m ! ?b = _ |- _] => rewrite H1 in H2; inv H2
+                  | [H: Some _ = Some _ |- _] => inv H
+                  | [|- context[(PTree.set ?k _ _) ! ?k]] => rewrite PTree.gss
+                  | [H: context[(PTree.set ?k _ _) ! ?k] |- _] => rewrite PTree.gss in H
+                  | [|- context[(PTree.set _ _ _) ! _]] => rewrite PTree.gsspec
+                  | [H: context[(PTree.set _ _ _) ! _] |- _] => rewrite PTree.gsspec in H
+                  | [|- context[peq ?a ?b]] => destruct (peq a b)
+                  | [H: context[peq ?a ?b] |- _] => destruct (peq a b)
+                  | [H: context[match ?x with | Some _ => _ | None => _ end] |- _] =>
+                    let H := fresh "H" in destruct x eqn:H
+                  | [|- context[match ?x with | Some _ => _ | None => _ end]] =>
+                    let H := fresh "H" in destruct x eqn:H
+                  | [H: False |- _] => inv H
+                  | [g: globdef _ _ |- _] => destruct g
+                end; subst; auto).
+  destruct p as [defs main]. unfold Genv.globalenv. simpl in *.
+  unfold Genv.add_globals. rewrite <- fold_left_rev_right.
+  unfold Genv.find_symbol, Genv.find_funct_ptr, Genv.find_var_info.
+  induction (rev defs); simpl.
+  { rewrite PTree.gempty. auto. }
+  rewrite ? PTree.gsspec. destruct a. simpl. destruct (peq i i0); [subst|]; simpl.
+  { destruct g; clarify.
+    - apply Genv.genv_vars_range in H3. xomega.
+    - apply Genv.genv_vars_range in H3. xomega.
+    - apply Genv.genv_vars_range in H1. xomega.
+    - apply Genv.genv_funs_range in H3. xomega.
+    - apply Genv.genv_funs_range in H3. xomega.
+    - apply Genv.genv_funs_range in H1. xomega.
+  }
+  { clarify.
+    - apply Genv.genv_funs_range in H1. xomega.
+    - apply Genv.genv_funs_range in H1. xomega.
+    - apply Genv.genv_funs_range in H1. xomega.
+    - apply Genv.genv_vars_range in H2. xomega.
+    - apply Genv.genv_vars_range in H2. xomega.
+    - apply Genv.genv_vars_range in H2. xomega.
+  }
+Qed.
+
 Lemma classify_call_correct:
   forall sp e m a v fd,
   Cminor.eval_expr ge sp e m a v ->
@@ -290,6 +401,83 @@ Proof.
   destruct (ef_inline e0). auto. exists b; auto.
   simpl in H0. discriminate.
   auto.
+Qed.
+
+Lemma classify_call_correct_ext:
+  forall sp e m a v fd sprog
+  (SPROG: program_linkeq Language_Cminor sprog prog),
+  Cminor.eval_expr ge sp e m a v ->
+  Genv.find_funct ge v = Some fd ->
+  match classify_call (Genv.globalenv sprog) a with
+  | Call_default => True
+  | Call_imm id => exists b, Genv.find_symbol ge id = Some b /\ v = Vptr b Int.zero
+  | Call_builtin ef => fd = External ef
+  end.
+Proof.
+  intros. exploit classify_call_correct; eauto.
+  unfold ge, tge in *. clear ge tge.
+  unfold classify_call. destruct (expr_is_addrof_ident a) eqn:Hident; auto.
+  destruct SPROG as [SPROG _]. unfold Cminor.fundef in *. simpl in *.
+  generalize (find_symbol_spec prog i).
+  generalize (find_symbol_spec sprog i).
+  unfold Cminor.fundef in *.
+  destruct (Genv.find_symbol (Genv.globalenv sprog) i) as [b_src|] eqn:Hb_src.
+  - match goal with
+      | [|- context[match ?g with | Some _ => _ | None => _ end -> _]] =>
+        let H := fresh "H" in destruct g as [g_src|] eqn:H; [|intro X; inv X]
+    end.
+    exploit (SPROG i); [rewrite PTree_guespec; apply H1|]. intros [g_tgt [Hg_tgt Hsim]].
+    rewrite PTree_guespec in Hg_tgt. unfold ident, Cminor.fundef in *. simpl in *. rewrite Hg_tgt.
+    inv Hsim.
+    + destruct (Genv.find_funct_ptr (Genv.globalenv sprog) b_src) eqn:Hfd_src; [|intro X; inv X].
+      destruct (Genv.find_var_info (Genv.globalenv sprog) b_src) eqn:Hvi_src; [intro X; inv X|].
+      intro. subst. fold Cminor.fundef in *.
+      destruct (Genv.find_symbol (Genv.globalenv prog) i) eqn:Hb_tgt; [|intro X; inv X].
+      destruct (Genv.find_funct_ptr (Genv.globalenv prog) b) eqn:Hfd'_src; [|intro X; inv X].
+      destruct (Genv.find_var_info (Genv.globalenv prog) b) eqn:Hvi'_src; [intro X; inv X|].
+      intro. subst. fold Cminor.fundef in *.
+      inv Hv; auto. inv H2.
+      * destruct f; inv H3. destruct f0; inv H4. destruct e1; inv Hlinkable. auto.
+      * destruct f; inv H3. destruct f0; inv H4. auto.
+    + destruct (Genv.find_funct_ptr (Genv.globalenv sprog) b_src) eqn:Hfd_src; [intro X; inv X|].
+      destruct (Genv.find_var_info (Genv.globalenv sprog) b_src) eqn:Hvi_src; [|intro X; inv X].
+      intro. subst. fold Cminor.fundef in *.
+      destruct (Genv.find_symbol (Genv.globalenv prog) i) eqn:Hb_tgt; [|intro X; inv X].
+      destruct (Genv.find_funct_ptr (Genv.globalenv prog) b) eqn:Hfd'_src; [intro X; inv X|].
+      destruct (Genv.find_var_info (Genv.globalenv prog) b) eqn:Hvi'_src; [|intro X; inv X].
+      intros ? [b' [Hb' Hv']]. subst. rewrite Hb_tgt in Hb'. inv Hb'.
+      eexists. split; eauto.
+  - match goal with
+      | [|- context[match ?g with | Some _ => _ | None => _ end -> _]] =>
+        let H := fresh "H" in destruct g as [g_src|] eqn:H; intro X; inv X
+    end.
+    fold Cminor.fundef in *.
+    destruct (Genv.find_symbol (Genv.globalenv prog) i) eqn:Hb_tgt.
+    { match goal with
+        | [|- context[match ?g with | Some _ => _ | None => _ end -> _]] =>
+          let H := fresh "H" in destruct g as [g_tgt|] eqn:H; [|intro X; inv X]
+      end.
+      destruct g_tgt as [fd_tgt|vi_tgt].
+      { destruct (Genv.find_funct_ptr (Genv.globalenv prog) b) eqn:Hfd_tgt; [|intro X; inv X].
+        destruct (Genv.find_var_info (Genv.globalenv prog) b) eqn:Hvi_tgt; [intro X; inv X|].
+        intro. subst. destruct f.
+        { rewrite Hb_tgt. auto. }
+        { destruct (ef_inline e0) eqn:Hinline.
+          { intro. subst. eexists. split; eauto.
+            destruct a; inv Hident. destruct c; inv H4. destruct (Int.eq i1 Int.zero); inv H5.
+            destruct v; inv H0. destruct (Int.eq_dec i0 Int.zero); inv H4.
+            inv H. inv H4. unfold Cminor.fundef in *. simpl in *. rewrite Hb_tgt in *.
+            inv H0. auto.
+          }
+          { rewrite Hb_tgt. auto. }
+        }
+      }
+      { destruct (Genv.find_funct_ptr (Genv.globalenv prog) b); [intro X; inv X|].
+        destruct (Genv.find_var_info (Genv.globalenv prog) b) eqn:Hvi_tgt; [|intro X; inv X].
+        intro. subst. rewrite Hb_tgt. auto.
+      }
+    }
+    { rewrite Hb_tgt. auto. }
 Qed.
 
 (** Translation of [switch] statements *)
@@ -589,30 +777,35 @@ Qed.
 Inductive match_cont: Cminor.cont -> CminorSel.cont -> Prop :=
   | match_cont_stop:
       match_cont Cminor.Kstop Kstop
-  | match_cont_seq: forall s s' k k',
-      sel_stmt ge s = OK s' ->
+  | match_cont_seq: forall s s' k k' sprog,
+      sel_stmt (Genv.globalenv sprog) s = OK s' ->
+      forall (SPROG: program_linkeq Language_Cminor sprog prog),
       match_cont k k' ->
       match_cont (Cminor.Kseq s k) (Kseq s' k')
   | match_cont_block: forall k k',
       match_cont k k' ->
       match_cont (Cminor.Kblock k) (Kblock k')
-  | match_cont_call: forall id f sp e k f' e' k',
-      sel_function ge f = OK f' ->
+  | match_cont_call: forall id f sp e k f' e' k' sprog,
+      sel_function (Genv.globalenv sprog) f = OK f' ->
+      forall (SPROG: program_linkeq Language_Cminor sprog prog),
       match_cont k k' -> env_lessdef e e' ->
       match_cont (Cminor.Kcall id f sp e k) (Kcall id f' sp e' k').
 
 Inductive match_states: Cminor.state -> CminorSel.state -> Prop :=
-  | match_state: forall f f' s k s' k' sp e m e' m'
-        (TF: sel_function ge f = OK f')
-        (TS: sel_stmt ge s = OK s')
+  | match_state: forall f f' s k s' k' sp e m e' m' sprog1 sprog2
+        (TF: sel_function (Genv.globalenv sprog1) f = OK f')
+        (TS: sel_stmt (Genv.globalenv sprog2) s = OK s')
+        (SPROG1: program_linkeq Language_Cminor sprog1 prog)
+        (SPROG2: program_linkeq Language_Cminor sprog2 prog)
         (MC: match_cont k k')
         (LD: env_lessdef e e')
         (ME: Mem.extends m m'),
       match_states
         (Cminor.State f s k sp e m)
         (State f' s' k' sp e' m')
-  | match_callstate: forall f f' args args' k k' m m'
-        (TF: sel_fundef ge f = OK f')
+  | match_callstate: forall f f' args args' k k' m m' sprog
+        (TF: sel_fundef (Genv.globalenv sprog) f = OK f')
+        (SPROG: program_linkeq Language_Cminor sprog prog)
         (MC: match_cont k k')
         (LD: Val.lessdef_list args args')
         (ME: Mem.extends m m'),
@@ -626,8 +819,9 @@ Inductive match_states: Cminor.state -> CminorSel.state -> Prop :=
       match_states
         (Cminor.Returnstate v k m)
         (Returnstate v' k' m')
-  | match_builtin_1: forall ef args args' optid f sp e k m al f' e' k' m'
-        (TF: sel_function ge f = OK f')
+  | match_builtin_1: forall ef args args' optid f sp e k m al f' e' k' m' sprog
+        (TF: sel_function (Genv.globalenv sprog) f = OK f')
+        (SPROG: program_linkeq Language_Cminor sprog prog)
         (MC: match_cont k k')
         (LDA: Val.lessdef_list args args')
         (LDE: env_lessdef e e')
@@ -636,8 +830,9 @@ Inductive match_states: Cminor.state -> CminorSel.state -> Prop :=
       match_states
         (Cminor.Callstate (External ef) args (Cminor.Kcall optid f sp e k) m)
         (State f' (Sbuiltin optid ef al) k' sp e' m')
-  | match_builtin_2: forall v v' optid f sp e k m f' e' m' k'
-        (TF: sel_function ge f = OK f')
+  | match_builtin_2: forall v v' optid f sp e k m f' e' m' k' sprog
+        (TF: sel_function (Genv.globalenv sprog) f = OK f')
+        (SPROG: program_linkeq Language_Cminor sprog prog)
         (MC: match_cont k k')
         (LDV: Val.lessdef v v')
         (LDE: env_lessdef e e')
@@ -649,40 +844,41 @@ Inductive match_states: Cminor.state -> CminorSel.state -> Prop :=
 Remark call_cont_commut:
   forall k k', match_cont k k' -> match_cont (Cminor.call_cont k) (call_cont k').
 Proof.
-  induction 1; simpl; auto. constructor. constructor; auto.
+  induction 1; simpl; auto. constructor. econstructor; eauto.
 Qed.
 
 Remark find_label_commut:
-  forall lbl s k s' k',
+  forall lbl s k s' k' sprog,
   match_cont k k' ->
-  sel_stmt ge s = OK s' ->
+  sel_stmt (Genv.globalenv sprog) s = OK s' ->
+  forall (SPROG: program_linkeq Language_Cminor sprog prog),
   match Cminor.find_label lbl s k, find_label lbl s' k' with
   | None, None => True
-  | Some(s1, k1), Some(s1', k1') => sel_stmt ge s1 = OK s1' /\ match_cont k1 k1'
+  | Some(s1, k1), Some(s1', k1') => sel_stmt (Genv.globalenv sprog) s1 = OK s1' /\ match_cont k1 k1'
   | _, _ => False
   end.
 Proof.
-  induction s; intros until k'; simpl; intros MC SE; try (monadInv SE); simpl; auto.
+  induction s; intros until sprog; simpl; intros MC SE SPROG; try (monadInv SE); simpl; auto.
 (* store *)
   unfold store. destruct (addressing m (sel_expr e)); simpl; auto.
 (* call *)
-  destruct (classify_call ge e); simpl; auto.
+  destruct (classify_call (Genv.globalenv sprog) e); simpl; auto.
 (* tailcall *)
-  destruct (classify_call ge e); simpl; auto.
+  destruct (classify_call (Genv.globalenv sprog) e); simpl; auto.
 (* seq *)
-  exploit (IHs1 (Cminor.Kseq s2 k)). constructor; eauto. eauto.  
+  exploit (IHs1 (Cminor.Kseq s2 k)); eauto. econstructor; eauto.  
   destruct (Cminor.find_label lbl s1 (Cminor.Kseq s2 k)) as [[sx kx] | ];
   destruct (find_label lbl x (Kseq x0 k')) as [[sy ky] | ];
-  intuition. apply IHs2; auto.
+  intuition. eapply IHs2; eauto.
 (* ifthenelse *)
   exploit (IHs1 k); eauto. 
   destruct (Cminor.find_label lbl s1 k) as [[sx kx] | ];
   destruct (find_label lbl x k') as [[sy ky] | ];
-  intuition. apply IHs2; auto.
+  intuition. eapply IHs2; eauto.
 (* loop *)
-  apply IHs. constructor; auto. simpl; rewrite EQ; auto. auto.
+  eapply IHs; eauto. econstructor; eauto. simpl; rewrite EQ; auto.
 (* block *)
-  apply IHs. constructor; auto. auto.
+  eapply IHs; eauto. constructor; auto.
 (* switch *)
   destruct b. 
   destruct (validate_switch Int64.modulus n l (compile_switch Int64.modulus n l)); inv SE.
@@ -710,9 +906,9 @@ Lemma sel_step_correct:
 Proof.
   induction 1; intros T1 ME; inv ME; try (monadInv TS).
 - (* skip seq *)
-  inv MC. left; econstructor; split. econstructor. constructor; auto.
+  inv MC. left; econstructor; split. econstructor. econstructor; eauto.
 - (* skip block *)
-  inv MC. left; econstructor; split. econstructor. constructor; auto.
+  inv MC. left; econstructor; split. econstructor. econstructor; eauto.
 - (* skip call *)
   exploit Mem.free_parallel_extends; eauto. intros [m2' [A B]].
   left; econstructor; split. 
@@ -722,35 +918,37 @@ Proof.
   constructor; auto.
 - (* assign *)
   exploit sel_expr_correct; eauto. intros [v' [A B]].
+  unfold sel_function in TF.
   left; econstructor; split.
   econstructor; eauto.
-  constructor; auto. apply set_var_lessdef; auto.
+  econstructor; eauto. apply set_var_lessdef; auto.
 - (* store *)
   exploit sel_expr_correct. eexact H. eauto. eauto. intros [vaddr' [A B]].
   exploit sel_expr_correct. eexact H0. eauto. eauto. intros [v' [C D]].
   exploit Mem.storev_extends; eauto. intros [m2' [P Q]].
   left; econstructor; split.
   eapply eval_store; eauto.
-  constructor; auto.
+  econstructor; eauto.
 - (* Scall *)
   exploit sel_exprlist_correct; eauto. intros [vargs' [C D]].
-  exploit classify_call_correct; eauto. 
-  destruct (classify_call ge a) as [ | id | ef].
+  exploit classify_call_correct_ext; eauto. 
+  simpl. fold Cminor.fundef.
+  destruct (classify_call (Genv.globalenv sprog2) a) as [ | id | ef].
 + (* indirect *)
   exploit sel_expr_correct; eauto. intros [vf' [A B]].
-  exploit functions_translated; eauto. intros (fd' & U & V).
+  exploit functions_translated; eauto. intros (fd' & U & sprog' & SPROG' & V).
   left; econstructor; split.
   econstructor; eauto. econstructor; eauto. 
-  apply sig_function_translated; auto.
-  constructor; auto. constructor; auto.
+  eapply sig_function_translated; eauto.
+  econstructor; eauto. econstructor; eauto.
 + (* direct *)
   intros [b [U V]]. 
-  exploit functions_translated; eauto. intros (fd' & X & Y).
+  exploit functions_translated; eauto. intros (fd' & X & sprog' & SPROG' & Y).
   left; econstructor; split.
   econstructor; eauto.
   subst vf. econstructor; eauto. rewrite symbols_preserved; eauto.
-  apply sig_function_translated; auto.
-  constructor; auto. constructor; auto.
+  eapply sig_function_translated; eauto.
+  econstructor; eauto. econstructor; eauto.
 + (* turned into Sbuiltin *)
   intros EQ. subst fd. 
   right; split. simpl. omega. split. auto. 
@@ -760,15 +958,16 @@ Proof.
   erewrite <- stackspace_function_translated in P by eauto.
   exploit sel_expr_correct; eauto. intros [vf' [A B]].
   exploit sel_exprlist_correct; eauto. intros [vargs' [C D]].
-  exploit functions_translated; eauto. intros [fd' [E F]].
+  exploit functions_translated; eauto. intros [fd' [E [sprog' [SPROG' F]]]].
   left; econstructor; split.
-  exploit classify_call_correct; eauto. 
-  destruct (classify_call ge a) as [ | id | ef]; intros. 
-  econstructor; eauto. econstructor; eauto. apply sig_function_translated; auto.
+  exploit classify_call_correct_ext; try apply SPROG2; eauto. 
+  simpl in *. fold Cminor.fundef in *.
+  destruct (classify_call (Genv.globalenv sprog2) a) as [ | id | ef]; intros. 
+  econstructor; eauto. econstructor; eauto. eapply sig_function_translated; eauto.
   destruct H2 as [b [U V]]. subst vf. inv B. 
-  econstructor; eauto. econstructor; eauto. rewrite symbols_preserved; eauto. apply sig_function_translated; auto.
-  econstructor; eauto. econstructor; eauto. apply sig_function_translated; auto.
-  constructor; auto. apply call_cont_commut; auto.
+  econstructor; eauto. econstructor; eauto. rewrite symbols_preserved; eauto. eapply sig_function_translated; eauto.
+  econstructor; eauto. econstructor; eauto. eapply sig_function_translated; eauto.
+  econstructor; eauto. apply call_cont_commut; auto.
 - (* Sbuiltin *)
   exploit sel_exprlist_correct; eauto. intros [vargs' [P Q]].
   exploit external_call_mem_extends; eauto. 
@@ -776,28 +975,28 @@ Proof.
   left; econstructor; split.
   econstructor. eauto. eapply external_call_symbols_preserved; eauto.
   exact symbols_preserved. exact varinfo_preserved.
-  constructor; auto.
+  econstructor; eauto.
   destruct optid; simpl; auto. apply set_var_lessdef; auto.
 - (* Seq *)
   left; econstructor; split.
-  constructor. constructor; auto. constructor; auto.
+  constructor. econstructor; eauto. econstructor; eauto.
 - (* Sifthenelse *)
   exploit sel_expr_correct; eauto. intros [v' [A B]].
   assert (Val.bool_of_val v' b). inv B. auto. inv H0.
   left; exists (State f' (if b then x else x0) k' sp e' m'); split.
   econstructor; eauto. eapply eval_condexpr_of_expr; eauto. 
-  constructor; auto. destruct b; auto.
+  econstructor; eauto. destruct b; auto.
 - (* Sloop *)
-  left; econstructor; split. constructor. constructor; auto.
-  constructor; auto. simpl; rewrite EQ; auto.
+  left; econstructor; split. constructor. econstructor; eauto.
+  econstructor; eauto. simpl; rewrite EQ; auto.
 - (* Sblock *)
-  left; econstructor; split. constructor. constructor; auto. constructor; auto.
+  left; econstructor; split. constructor. econstructor; eauto. constructor; auto.
 - (* Sexit seq *)
-  inv MC. left; econstructor; split. constructor. constructor; auto.
+  inv MC. left; econstructor; split. constructor. econstructor; eauto.
 - (* Sexit0 block *)
-  inv MC. left; econstructor; split. constructor. constructor; auto.
+  inv MC. left; econstructor; split. constructor. econstructor; eauto.
 - (* SexitS block *)
-  inv MC. left; econstructor; split. constructor. constructor; auto.
+  inv MC. left; econstructor; split. constructor. econstructor; eauto.
 - (* Sswitch *)
   inv H0; simpl in TS.
 + set (ct := compile_switch Int.modulus default cases) in *.
@@ -805,13 +1004,13 @@ Proof.
   exploit sel_expr_correct; eauto. intros [v' [A B]]. inv B.
   left; econstructor; split. 
   econstructor. eapply sel_switch_int_correct; eauto. 
-  constructor; auto.
+  econstructor; eauto.
 + set (ct := compile_switch Int64.modulus default cases) in *.
   destruct (validate_switch Int64.modulus default cases ct) eqn:VALID; inv TS.
   exploit sel_expr_correct; eauto. intros [v' [A B]]. inv B.
   left; econstructor; split.
-  econstructor. eapply sel_switch_long_correct; eauto. 
-  constructor; auto.
+  econstructor. eapply sel_switch_long_correct; eauto.
+  econstructor; eauto.
 - (* Sreturn None *)
   exploit Mem.free_parallel_extends; eauto. intros [m2' [P Q]].
   erewrite <- stackspace_function_translated in P by eauto.
@@ -826,26 +1025,26 @@ Proof.
   econstructor; eauto.
   constructor; auto. apply call_cont_commut; auto.
 - (* Slabel *)
-  left; econstructor; split. constructor. constructor; auto.
+  left; econstructor; split. constructor. econstructor; eauto.
 - (* Sgoto *)
-  assert (sel_stmt ge (Cminor.fn_body f) = OK (fn_body f')).
+  assert (sel_stmt (Genv.globalenv sprog1) (Cminor.fn_body f) = OK (fn_body f')).
   { monadInv TF; simpl; auto. }
   exploit (find_label_commut lbl (Cminor.fn_body f) (Cminor.call_cont k)).
-    apply call_cont_commut; eauto. eauto.
+    apply call_cont_commut; eauto. eauto. auto. auto.
   rewrite H. 
   destruct (find_label lbl (fn_body f') (call_cont k'0))
   as [[s'' k'']|] eqn:?; intros; try contradiction.
   destruct H1. 
   left; econstructor; split.
   econstructor; eauto. 
-  constructor; auto.
+  econstructor; eauto.
 - (* internal function *)
   monadInv TF. generalize EQ; intros TF; monadInv TF.
   exploit Mem.alloc_extends. eauto. eauto. apply Zle_refl. apply Zle_refl. 
   intros [m2' [A B]].
   left; econstructor; split.
   econstructor; simpl; eauto.
-  constructor; simpl; auto. apply set_locals_lessdef. apply set_params_lessdef; auto.
+  econstructor; simpl; eauto. apply set_locals_lessdef. apply set_params_lessdef; auto.
 - (* external call *)
   monadInv TF.
   exploit external_call_mem_extends; eauto. 
@@ -860,14 +1059,14 @@ Proof.
   left; econstructor; split.
   econstructor. eauto. eapply external_call_symbols_preserved; eauto.
   exact symbols_preserved. exact varinfo_preserved.
-  constructor; auto.
+  econstructor; eauto.
 - (* return *)
   inv MC. 
   left; econstructor; split. 
   econstructor. 
-  constructor; auto. destruct optid; simpl; auto. apply set_var_lessdef; auto.
+  econstructor; eauto. destruct optid; simpl; auto. apply set_var_lessdef; auto.
 - (* return of an external call turned into a Sbuiltin *)
-  right; split. simpl; omega. split. auto. constructor; auto. 
+  right; split. simpl; omega. split. auto. econstructor; eauto. 
   destruct optid; simpl; auto. apply set_var_lessdef; auto.
 Qed.
 
@@ -876,15 +1075,16 @@ Lemma sel_initial_states:
   exists R, initial_state tprog R /\ match_states S R.
 Proof.
   induction 1.
-  exploit function_ptr_translated; eauto. intros (f' & A & B).
+  exploit function_ptr_translated; eauto. intros (f' & A & sprog & SPROG & B).
   econstructor; split.
   econstructor.
-  eapply Genv.init_mem_transf_partial; eauto.
-  simpl. fold tge. rewrite symbols_preserved.
-  erewrite transform_partial_program_main by eauto. eexact H0.
-  eauto.
-  rewrite <- H2. apply sig_function_translated; auto.
-  constructor; auto. constructor. apply Mem.extends_refl.
+  exploit Genv.init_mem_match; eauto.
+  replace (prog_main tprog) with (prog_main prog).
+  rewrite symbols_preserved. eauto.
+  inv TRANSF. auto.
+  exploit function_ptr_translated; eauto.
+  rewrite <- H2. eapply sig_function_translated; eauto.
+  econstructor; eauto. constructor. apply Mem.extends_refl.
 Qed.
 
 Lemma sel_final_states:
@@ -892,6 +1092,16 @@ Lemma sel_final_states:
   match_states S R -> Cminor.final_state S r -> final_state R r.
 Proof.
   intros. inv H0. inv H. inv MC. inv LD. constructor.
+Qed.
+
+Theorem transl_program_correct:
+  forward_simulation (Cminor.semantics prog) (CminorSel.semantics tprog).
+Proof.
+  apply forward_simulation_opt with (match_states := match_states) (measure := measure). 
+  eapply symbols_preserved; eauto.
+  apply sel_initial_states; auto.
+  apply sel_final_states; auto.
+  apply sel_step_correct; auto.
 Qed.
 
 End PRESERVATION.
@@ -919,16 +1129,135 @@ Proof.
   destruct H1. subst a1. eapply check_helper_correct; eauto. eauto. 
 Qed.
 
-Theorem transf_program_correct:
-  forall prog tprog,
-  sel_program prog = OK tprog ->
-  forward_simulation (Cminor.semantics prog) (CminorSel.semantics tprog).
+Lemma link_program_check_helper
+      idsig p1 p2 p
+      (LINK: link_program Language_Cminor p1 p2 = Some p)
+      (CHECK1: SelectLong.check_helper (Genv.globalenv p1) idsig = OK tt)
+      (CHECK2: SelectLong.check_helper (Genv.globalenv p2) idsig = OK tt):
+  SelectLong.check_helper (Genv.globalenv p) idsig = OK tt.
 Proof.
-  intros. unfold sel_program in H. set (ge := Genv.globalenv prog) in *.
-  destruct (check_helpers ge) eqn:CH; simpl in H; try discriminate.
-  apply forward_simulation_opt with (match_states := match_states prog tprog) (measure := measure). 
-  eapply symbols_preserved; eauto.
-  apply sel_initial_states; auto.
-  apply sel_final_states; auto.
-  apply sel_step_correct; auto. eapply check_helpers_correct; eauto.
+  destruct idsig as [id sig]. simpl in *.
+  destruct (@Genv.find_symbol Cminor.fundef unit (Genv.globalenv p1) id) as [s1|] eqn:SYM1; try congruence.
+  destruct (@Genv.find_symbol Cminor.fundef unit (Genv.globalenv p2) id) as [s2|] eqn:SYM2; try congruence.
+  destruct (@Genv.find_funct_ptr Cminor.fundef unit (Genv.globalenv p1) s1) as [f1|] eqn:FUNC1; try congruence.
+  destruct (@Genv.find_funct_ptr Cminor.fundef unit (Genv.globalenv p2) s2) as [f2|] eqn:FUNC2; try congruence.
+  destruct f1 as [|[]]; try congruence.
+  destruct f2 as [|[]]; try congruence.
+  destruct (ident_eq name id); simpl in *; subst; try congruence.
+  destruct (signature_eq sg sig); simpl in *; subst; try congruence.
+  destruct (ident_eq name0 id); simpl in *; subst; try congruence.
+  destruct (signature_eq sg0 sig); simpl in *; subst; try congruence.
+  exploit find_symbol_spec; eauto.
+  instantiate (1 := p1). instantiate (1 := id).
+  simpl in *. fold Cminor.fundef in *. rewrite SYM1, FUNC1.
+  intro ID1.
+  exploit find_symbol_spec; eauto.
+  instantiate (1 := p2). instantiate (1 := id).
+  simpl in *. fold Cminor.fundef in *. rewrite SYM2, FUNC2.
+  intro ID2.
+  exploit find_symbol_spec; eauto.
+  instantiate (1 := p). instantiate (1 := id).
+  simpl in *. fold Cminor.fundef in *.
+  intro ID.
+  unfold link_program in LINK. simpl in *. fold Cminor.fundef in *.
+  destruct (Pos.eqb (prog_main p1) (prog_main p2)); try congruence.
+  destruct (link_globdef_list Language_Cminor (prog_defs p1) (prog_defs p2)) eqn:DEFS; inv LINK.
+  unfold link_globdef_list in DEFS. simpl in *. fold Cminor.fundef in *.
+  destruct (link_globdefs Language_Cminor (PTree_unelements (prog_defs p1)) (PTree_unelements (prog_defs p2))) eqn:DEFS'; inv DEFS.
+  exploit gtlink_globdefs; eauto. instantiate (1 := id). rewrite ? PTree_guespec.
+  revert ID1 ID2. simpl in *. fold Cminor.fundef in *. fold ident.
+  destruct
+    (@option_map (prod ident (globdef Cminor.fundef unit))
+                 (globdef Cminor.fundef unit) (@snd ident (globdef Cminor.fundef unit))
+                 (@find (prod ident (globdef Cminor.fundef unit))
+                        (fun id0 : prod ident (globdef Cminor.fundef unit) =>
+                           @proj_sumbool
+                             (@eq ident id (@fst ident (globdef Cminor.fundef unit) id0))
+                             (not
+                                (@eq ident id (@fst ident (globdef Cminor.fundef unit) id0)))
+                             (peq id (@fst ident (globdef Cminor.fundef unit) id0)))
+                        (@rev (prod ident (globdef Cminor.fundef unit))
+                              (@prog_defs Cminor.fundef unit p1)))); [|intros; exfalso; auto].
+  destruct
+    (@option_map (prod ident (globdef Cminor.fundef unit))
+                 (globdef Cminor.fundef unit) (@snd ident (globdef Cminor.fundef unit))
+                 (@find (prod ident (globdef Cminor.fundef unit))
+                        (fun id0 : prod ident (globdef Cminor.fundef unit) =>
+                           @proj_sumbool
+                             (@eq ident id (@fst ident (globdef Cminor.fundef unit) id0))
+                             (not
+                                (@eq ident id (@fst ident (globdef Cminor.fundef unit) id0)))
+                             (peq id (@fst ident (globdef Cminor.fundef unit) id0)))
+                        (@rev (prod ident (globdef Cminor.fundef unit))
+                              (@prog_defs Cminor.fundef unit p2)))); [|intros; exfalso; auto].
+  destruct g, g0; intros; try (exfalso; auto; fail).
+  destruct (t ! id) eqn:TID; [|exfalso; auto].
+  rewrite PTree_gespec in TID.
+  rewrite <- list_norepet_option_map_find in TID; [|apply PTree.elements_keys_norepet].
+  simpl in *. fold Cminor.fundef ident in *. rewrite TID in ID.
+  destruct (Genv.find_symbol (Genv.globalenv {| prog_defs := PTree.elements t; prog_main := prog_main p1 |}) id); [|exfalso; auto].
+  destruct g; [|destruct H as [[]|[]]; congruence].
+  destruct (Genv.find_funct_ptr (Genv.globalenv {| prog_defs := PTree.elements t; prog_main := prog_main p1 |}) b); [|exfalso; auto].
+  destruct (Genv.find_var_info (Genv.globalenv {| prog_defs := PTree.elements t; prog_main := prog_main p1 |}) b); [exfalso; auto|].
+  destruct (Genv.find_var_info (Genv.globalenv p1) s1); [exfalso; auto|].
+  destruct (Genv.find_var_info (Genv.globalenv p2) s2); [exfalso; auto|].
+  subst. destruct H as [[]|[]]; inv H0.
+  - destruct (ident_eq id id); [|congruence].
+    destruct (signature_eq sig sig); [|congruence].
+    auto.
+  - destruct (ident_eq id id); [|congruence].
+    destruct (signature_eq sig sig); [|congruence].
+    auto.
+Qed.
+
+Lemma link_program_check_helpers
+      p1 p2 p
+      (LINK: link_program Language_Cminor p1 p2 = Some p)
+      (CHECK1: SelectLong.check_helpers (Genv.globalenv p1) = OK tt)
+      (CHECK2: SelectLong.check_helpers (Genv.globalenv p2) = OK tt):
+  SelectLong.check_helpers (Genv.globalenv p) = OK tt.
+Proof.
+  unfold SelectLong.check_helpers in *.
+  monadInv CHECK1. monadInv CHECK2.
+  apply mmap_inversion in EQ. apply mmap_inversion in EQ0.
+  revert x x0 EQ EQ0. induction SelectLong.i64_helpers; intros; auto.
+  inv EQ. inv EQ0. destruct b0, b1. simpl.
+  erewrite link_program_check_helper; eauto. simpl.
+  exploit IHl; eauto. simpl in *.
+  destruct (mmap (SelectLong.check_helper (Genv.globalenv p)) l); auto.
+Qed.
+
+Lemma Selection_sepcomp_rel
+      cminorprog cminorselprog
+      (Htrans: Selection.sel_program cminorprog = OK cminorselprog):
+  @sepcomp_rel
+    Language.Language_Cminor Language.Language_CminorSel
+    (fun p f tf => Selection.sel_function (Genv.globalenv p) f = OK tf)
+    (fun p ef tef => ef = tef)
+    (@OK _)
+    cminorprog cminorselprog.
+Proof.
+  monadInv Htrans.
+  destruct cminorprog as [defs ?], cminorselprog as [tdefs ?].
+  unfold transform_partial_program, transform_partial_program2 in EQ0. monadInv EQ0.
+  constructor; auto. simpl in *.
+  revert tdefs EQ EQ1. generalize defs at 1 2 4 as fdefs.
+  induction defs; simpl; intros fdefs tdefs Hhelpers Hdefs.
+  { inv Hdefs. constructor. }
+  destruct a. destruct g.
+  - match goal with
+      | [H: match ?x with OK _ => _ | Error _ => _ end = OK _ |- _] =>
+        destruct x as [tf|] eqn:Hf; [|inv H]
+    end.
+    monadInv Hdefs. constructor; simpl.
+    + split; auto. eexists. split; [reflexivity|].
+      destruct f; inv Hf.
+      * monadInv H0.
+        eapply (@grel_f Language.Language_Cminor Language.Language_CminorSel); simpl; auto.
+      * eapply (@grel_ef Language.Language_Cminor Language.Language_CminorSel); simpl; auto.
+    + apply IHdefs; auto.
+  - monadInv Hdefs. constructor; simpl.
+    + split; auto. eexists. split; [reflexivity|].
+      eapply (@grel_gv Language.Language_Cminor Language.Language_CminorSel); auto.
+    + apply IHdefs; auto.
 Qed.
