driver/Compilerproof.v
@@ -1,0 +1,216 @@
+(* *********************************************************************)
+(*                                                                     *)
+(*              The Compcert verified compiler                         *)
+(*                                                                     *)
+(*          Xavier Leroy, INRIA Paris-Rocquencourt                     *)
+(*                                                                     *)
+(*  Copyright Institut National de Recherche en Informatique et en     *)
+(*  Automatique.  All rights reserved.  This file is distributed       *)
+(*  under the terms of the INRIA Non-Commercial License Agreement.     *)
+(*                                                                     *)
+(* *********************************************************************)
+
+(** The whole compiler and its proof of semantic preservation *)
+
+(** Libraries. *)
+Require Import String.
+Require Import Coqlib.
+Require Import Errors.
+Require Import AST.
+Require Import Smallstep.
+(** Languages (syntax and semantics). *)
+Require Csyntax.
+Require Csem.
+Require Cstrategy.
+Require Cexec.
+Require Clight.
+Require Csharpminor.
+Require Cminor.
+Require CminorSel.
+Require RTL.
+Require LTL.
+Require Linear.
+Require Mach.
+Require Asm.
+(** Translation passes. *)
+Require Initializers.
+Require SimplExpr.
+Require SimplLocals.
+Require Cshmgen.
+Require Cminorgen.
+Require Selection.
+Require RTLgen.
+Require Tailcall.
+Require Inlining.
+Require Renumber.
+Require Constprop.
+Require CSE.
+Require Deadcode.
+Require Allocation.
+Require Tunneling.
+Require Linearize.
+Require CleanupLabels.
+Require Stacking.
+Require Asmgen.
+(** Proofs of semantic preservation. *)
+Require SimplExprproof.
+Require SimplLocalsproof.
+Require Cshmgenproof.
+Require Cminorgenproof.
+Require Selectionproof.
+Require RTLgenproof.
+Require Tailcallproof.
+Require Inliningproof.
+Require Renumberproof.
+Require Constpropproof.
+Require CSEproof.
+Require Deadcodeproof.
+Require Allocproof.
+Require Tunnelingproof.
+Require Linearizeproof.
+Require CleanupLabelsproof.
+Require Stackingproof.
+Require Asmgenproof.
+
+Require Import Compiler.
+
+(** * Semantic preservation *)
+
+(** We prove that the [transf_program] translations preserve semantics
+  by constructing the following simulations:
+- Forward simulations from [Cstrategy] / [Cminor] / [RTL] to [Asm]
+  (composition of the forward simulations for each pass).
+- Backward simulations for the same languages
+  (derived from the forward simulation, using receptiveness of the source
+  language and determinacy of [Asm]).
+- Backward simulation from [Csem] to [Asm]
+  (composition of two backward simulations).
+
+These results establish the correctness of the whole compiler! *)
+
+Theorem transf_rtl_program_correct:
+  forall p tp,
+  transf_rtl_program p = OK tp ->
+  forward_simulation (RTL.semantics p) (Asm.semantics tp)
+  * backward_simulation (RTL.semantics p) (Asm.semantics tp).
+Proof.
+  intros.
+  assert (F: forward_simulation (RTL.semantics p) (Asm.semantics tp)).
+  unfold transf_rtl_program, time in H.
+  repeat rewrite compose_print_identity in H.
+  simpl in H.
+  set (p1 := Tailcall.transf_program p) in *.
+  destruct (Inlining.transf_program p1) as [p11|] eqn:?; simpl in H; try discriminate.
+  set (p12 := Renumber.transf_program p11) in *.
+  set (p2 := Constprop.transf_program p12) in *.
+  set (p21 := Renumber.transf_program p2) in *.
+  destruct (CSE.transf_program p21) as [p3|] eqn:?; simpl in H; try discriminate.
+  destruct (Deadcode.transf_program p3) as [p31|] eqn:?; simpl in H; try discriminate.
+  destruct (Allocation.transf_program p31) as [p4|] eqn:?; simpl in H; try discriminate.
+  set (p5 := Tunneling.tunnel_program p4) in *.
+  destruct (Linearize.transf_program p5) as [p6|] eqn:?; simpl in H; try discriminate.
+  set (p7 := CleanupLabels.transf_program p6) in *.
+  destruct (Stacking.transf_program p7) as [p8|] eqn:?; simpl in H; try discriminate.
+  eapply compose_forward_simulation. apply Tailcallproof.transf_program_correct. 
+  eapply compose_forward_simulation. apply Inliningproof.transf_program_correct. apply Inliningproof.Inlining_sepcomp_rel. eassumption.
+  eapply compose_forward_simulation. apply Renumberproof.transf_program_correct.
+  eapply compose_forward_simulation. apply Constpropproof.transf_program_correct. apply Constpropproof.Constprop_sepcomp_rel. eauto.
+  eapply compose_forward_simulation. apply Renumberproof.transf_program_correct. 
+  eapply compose_forward_simulation. apply CSEproof.transf_program_correct. apply CSEproof.CSE_sepcomp_rel. eassumption.
+  eapply compose_forward_simulation. apply Deadcodeproof.transf_program_correct. apply Deadcodeproof.Deadcode_sepcomp_rel. eassumption.
+  eapply compose_forward_simulation. apply Allocproof.transf_program_correct. eassumption.
+  eapply compose_forward_simulation. apply Tunnelingproof.transf_program_correct.
+  eapply compose_forward_simulation. apply Linearizeproof.transf_program_correct. eassumption. 
+  eapply compose_forward_simulation. apply CleanupLabelsproof.transf_program_correct. 
+  eapply compose_forward_simulation. apply Stackingproof.transf_program_correct.
+    eexact Asmgenproof.return_address_exists. eassumption.
+  apply Asmgenproof.transf_program_correct; eauto.
+  split. auto. 
+  apply forward_to_backward_simulation. auto. 
+  apply RTL.semantics_receptive.
+  apply Asm.semantics_determinate.
+Qed.
+
+Theorem transf_cminor_program_correct:
+  forall p tp,
+  transf_cminor_program p = OK tp ->
+  forward_simulation (Cminor.semantics p) (Asm.semantics tp)
+  * backward_simulation (Cminor.semantics p) (Asm.semantics tp).
+Proof.
+  intros.
+  assert (F: forward_simulation (Cminor.semantics p) (Asm.semantics tp)).
+  unfold transf_cminor_program, time in H.
+  repeat rewrite compose_print_identity in H.
+  simpl in H. 
+  destruct (Selection.sel_program p) as [p1|] eqn:?; simpl in H; try discriminate.
+  destruct (RTLgen.transl_program p1) as [p2|] eqn:?; simpl in H; try discriminate.
+  eapply compose_forward_simulation. apply Selectionproof.transl_program_correct. monadInv Heqr. eapply Selectionproof.check_helpers_correct. eauto. apply Selectionproof.Selection_sepcomp_rel. eassumption.
+  eapply compose_forward_simulation. apply RTLgenproof.transf_program_correct. eassumption.
+  exact (fst (transf_rtl_program_correct _ _ H)).
+
+  split. auto. 
+  apply forward_to_backward_simulation. auto. 
+  apply Cminor.semantics_receptive.
+  apply Asm.semantics_determinate.
+Qed.
+
+Theorem transf_clight_program_correct:
+  forall p tp,
+  transf_clight_program p = OK tp ->
+  forward_simulation (Clight.semantics1 p) (Asm.semantics tp)
+  * backward_simulation (Clight.semantics1 p) (Asm.semantics tp).
+Proof.
+  intros. 
+  assert (F: forward_simulation (Clight.semantics1 p) (Asm.semantics tp)).
+  revert H; unfold transf_clight_program, time; simpl.
+  rewrite print_identity.
+  caseEq (SimplLocals.transf_program p); simpl; try congruence; intros p0 EQ0.
+  caseEq (Cshmgen.transl_program p0); simpl; try congruence; intros p1 EQ1.
+  caseEq (Cminorgen.transl_program p1); simpl; try congruence; intros p2 EQ2.
+  intros EQ3.
+  eapply compose_forward_simulation. apply SimplLocalsproof.transf_program_correct. eauto.
+  eapply compose_forward_simulation. apply Cshmgenproof.transl_program_correct. eauto.
+  eapply compose_forward_simulation. apply Cminorgenproof.transl_program_correct. eauto.
+  exact (fst (transf_cminor_program_correct _ _ EQ3)). 
+
+  split. auto. 
+  apply forward_to_backward_simulation. auto. 
+  apply Clight.semantics_receptive.
+  apply Asm.semantics_determinate.
+Qed.
+
+Theorem transf_cstrategy_program_correct:
+  forall p tp,
+  transf_c_program p = OK tp ->
+  forward_simulation (Cstrategy.semantics p) (Asm.semantics tp)
+  * backward_simulation (atomic (Cstrategy.semantics p)) (Asm.semantics tp).
+Proof.
+  intros.
+  assert (F: forward_simulation (Cstrategy.semantics p) (Asm.semantics tp)).
+  revert H; unfold transf_c_program, time; simpl.
+  caseEq (SimplExpr.transl_program p); simpl; try congruence; intros p0 EQ0.
+  intros EQ1.
+  eapply compose_forward_simulation. apply SimplExprproof.transl_program_correct. apply SimplExprproof.SimplExpr_sepcomp_rel. eauto.
+  exact (fst (transf_clight_program_correct _ _ EQ1)). 
+
+  split. auto. 
+  apply forward_to_backward_simulation.
+  apply factor_forward_simulation. auto. eapply sd_traces. eapply Asm.semantics_determinate.
+  apply atomic_receptive. apply Cstrategy.semantics_strongly_receptive.
+  apply Asm.semantics_determinate.
+Qed.
+
+Theorem transf_c_program_correct:
+  forall p tp,
+  transf_c_program p = OK tp ->
+  backward_simulation (Csem.semantics p) (Asm.semantics tp).
+Proof.
+  intros. 
+  apply compose_backward_simulation with (atomic (Cstrategy.semantics p)).
+  eapply sd_traces; eapply Asm.semantics_determinate.
+  apply factor_backward_simulation. 
+  apply Cstrategy.strategy_simulation.
+  apply Csem.semantics_single_events.
+  eapply ssr_well_behaved; eapply Cstrategy.semantics_strongly_receptive.
+  exact (snd (transf_cstrategy_program_correct _ _ H)).
+Qed.
