driver/Linkerproof.v
@@ -10,12 +10,13 @@ Require Import Tree.
 Require Import LinkerBasicproof Sig.
 Require Import SepcompRel.
 
-Require SimplExprproof_sepcomp.
-Require Selectionproof_sepcomp.
-Require Inliningproof_sepcomp.
-Require Constpropproof_sepcomp.
-Require CSEproof_sepcomp.
-Require Deadcodeproof_sepcomp.
+Require SimplExprproof.
+Require Selectionproof.
+Require Inliningproof.
+Require Constpropproof.
+Require CSEproof.
+Require Deadcodeproof.
+
 
 Set Implicit Arguments.
 
@@ -37,163 +38,6 @@ Proof.
   constructor; intros.
   - destruct H as [? [? ?]]. subst. auto.
   - destruct a; inv H. eexists. split; eauto.
-Qed.
-
-Lemma SimplExpr_sepcomp_rel
-      cprog clightprog
-      (Htrans: SimplExpr.transl_program cprog = OK clightprog):
-  @sepcomp_rel
-    Language_C Language_Clight
-    (fun _ f tf => SimplExprspec.tr_function f tf)
-    (fun _ ef tef => ef = tef)
-    (@OK _)
-    cprog clightprog.
-Proof.
-  destruct cprog as [defs ?], clightprog as [tdefs ?].
-  exploit SimplExprspec.transl_program_spec; eauto. clear Htrans.
-  intros [[tglob [Hmatch Htglob]] Hmain]. constructor; auto.
-  rewrite app_nil_r in *. simpl in *. subst.
-  eapply list_forall2_imply; eauto. intros. inv H1; simpl; split; auto.
-  - eexists. split; [reflexivity|].
-    inv H2.
-    + eapply (@grel_f Language_C Language_Clight); simpl; auto.
-    + eapply (@grel_ef Language_C Language_Clight); simpl; auto.
-  - eexists. split; [reflexivity|].
-    apply (@grel_gv Language_C Language_Clight). auto.
-Qed.
-
-Lemma Selection_sepcomp_rel
-      cminorprog cminorselprog
-      (Htrans: Selection.sel_program cminorprog = OK cminorselprog):
-  @sepcomp_rel
-    Language_Cminor Language_CminorSel
-    (fun p f tf => Selection.sel_function (Genv.globalenv p) f = OK tf)
-    (fun p ef tef => ef = tef)
-    (@OK _)
-    cminorprog cminorselprog.
-Proof.
-  monadInv Htrans.
-  destruct cminorprog as [defs ?], cminorselprog as [tdefs ?].
-  unfold transform_partial_program, transform_partial_program2 in EQ0. monadInv EQ0.
-  constructor; auto. simpl in *.
-  revert tdefs EQ EQ1. generalize defs at 1 2 4 as fdefs.
-  induction defs; simpl; intros fdefs tdefs Hhelpers Hdefs.
-  { inv Hdefs. constructor. }
-  destruct a. destruct g.
-  - match goal with
-      | [H: match ?x with OK _ => _ | Error _ => _ end = OK _ |- _] =>
-        destruct x as [tf|] eqn:Hf; [|inv H]
-    end.
-    monadInv Hdefs. constructor; simpl.
-    + split; auto. eexists. split; [reflexivity|].
-      destruct f; inv Hf.
-      * monadInv H0.
-        eapply (@grel_f Language_Cminor Language_CminorSel); simpl; auto.
-      * eapply (@grel_ef Language_Cminor Language_CminorSel); simpl; auto.
-    + apply IHdefs; auto.
-  - monadInv Hdefs. constructor; simpl.
-    + split; auto. eexists. split; [reflexivity|].
-      eapply (@grel_gv Language_Cminor Language_CminorSel); auto.
-    + apply IHdefs; auto.
-Qed.
-
-Lemma Tailcall_sepcomp_rel
-      rtlprog1 rtlprog2
-      (Htrans: Tailcall.transf_program rtlprog1 = rtlprog2):
-  @sepcomp_rel
-    Language_RTL Language_RTL
-    (fun p f tf => Tailcall.transf_function f = tf)
-    (fun p ef tef => ef = tef)
-    (@OK _)
-    rtlprog1 rtlprog2.
-Proof.
-  apply transf_program_sepcomp_rel. rewrite <- Htrans.
-  unfold Tailcall.transf_program. f_equal.
-  apply Axioms.functional_extensionality. intro fd.
-  destruct fd; auto.
-Qed.
-
-Lemma Inlining_sepcomp_rel
-      rtlprog1 rtlprog2
-      (Htrans: Inlining.transf_program rtlprog1 = OK rtlprog2):
-  @sepcomp_rel
-    Language_RTL Language_RTL
-    (fun p f tf => Inlining.transf_function (Inlining.funenv_program p) f = OK tf)
-    (fun p ef tef => (fun _ ef => OK ef) p ef = OK tef)
-    (@OK _)
-    rtlprog1 rtlprog2.
-Proof.
-  apply transf_partial_sepcomp_rel.
-  unfold progT, RTL.program, RTL.fundef in *. simpl in *. rewrite <- Htrans.
-  unfold Inlining.transf_program. f_equal.
-  apply Axioms.functional_extensionality. intro fd.
-  destruct fd; auto.
-Qed.
-
-Lemma Renumber_sepcomp_rel
-      rtlprog1 rtlprog2
-      (Htrans: Renumber.transf_program rtlprog1 = rtlprog2):
-  @sepcomp_rel
-    Language_RTL Language_RTL
-    (fun p f tf => Renumber.transf_function f = tf)
-    (fun p ef tef => ef = tef)
-    (@OK _)
-    rtlprog1 rtlprog2.
-Proof.
-  apply transf_program_sepcomp_rel. rewrite <- Htrans.
-  unfold Renumber.transf_program. f_equal.
-  apply Axioms.functional_extensionality. intro fd.
-  destruct fd; auto.
-Qed.
-
-Lemma Constprop_sepcomp_rel
-      rtlprog1 rtlprog2
-      (Htrans: Constprop.transf_program rtlprog1 = rtlprog2):
-  @sepcomp_rel
-    Language_RTL Language_RTL
-    (fun p f tf => Constprop.transf_function (ValueAnalysis.romem_for_program p) f = tf)
-    (fun p ef tef => ef = tef)
-    (@OK _)
-    rtlprog1 rtlprog2.
-Proof.
-  apply transf_program_sepcomp_rel. rewrite <- Htrans.
-  unfold Constprop.transf_program. f_equal.
-  apply Axioms.functional_extensionality. intro fd.
-  destruct fd; auto.
-Qed.
-
-Lemma CSE_sepcomp_rel
-      rtlprog1 rtlprog2
-      (Htrans: CSE.transf_program rtlprog1 = OK rtlprog2):
-  @sepcomp_rel
-    Language_RTL Language_RTL
-    (fun p f tf => CSE.transf_function (ValueAnalysis.romem_for_program p) f = OK tf)
-    (fun p ef tef => (fun _ ef => OK ef) p ef = OK tef)
-    (@OK _)
-    rtlprog1 rtlprog2.
-Proof.
-  apply transf_partial_sepcomp_rel.
-  unfold progT, RTL.program, RTL.fundef in *. simpl in *. rewrite <- Htrans.
-  unfold CSE.transf_program. f_equal.
-  apply Axioms.functional_extensionality. intro fd.
-  destruct fd; auto.
-Qed.
-
-Lemma Deadcode_sepcomp_rel
-      rtlprog1 rtlprog2
-      (Htrans: Deadcode.transf_program rtlprog1 = OK rtlprog2):
-  @sepcomp_rel
-    Language_RTL Language_RTL
-    (fun p f tf => Deadcode.transf_function (ValueAnalysis.romem_for_program p) f = OK tf)
-    (fun p ef tef => (fun _ ef => OK ef) p ef = OK tef)
-    (@OK _)
-    rtlprog1 rtlprog2.
-Proof.
-  apply transf_partial_sepcomp_rel.
-  unfold progT, RTL.program, RTL.fundef in *. simpl in *. rewrite <- Htrans.
-  unfold Deadcode.transf_program. f_equal.
-  apply Axioms.functional_extensionality. intro fd.
-  destruct fd; auto.
 Qed.
 
 Ltac clarify :=
@@ -226,41 +70,41 @@ Ltac simplify :=
 
 Lemma linker_correct_determinate_forward
         ctree asmtree cprog
-        (CLINK: Tree.reduce (link_program Language_C) ctree = Some cprog)
+        (CLINK: Tree.reduce (link_program Language.Language_C) ctree = Some cprog)
         (TRANSF: Tree.Forall2 (fun c a => transf_c_program c = OK a) ctree asmtree):
   exists (asmprog:Asm.program)
     (_:forward_simulation (Cstrategy.semantics cprog) (Asm.semantics asmprog)),
-    Tree.reduce (link_program Language_Asm) asmtree = Some asmprog.
+    Tree.reduce (link_program Language.Language_Asm) asmtree = Some asmprog.
 Proof.
   repeat intro.
 
   (* C *)
   unfold transf_c_program in TRANSF. clarify.
 
-  eapply Tree.Forall2_implies in T; [|apply SimplExpr_sepcomp_rel].
+  eapply Tree.Forall2_implies in T; [|apply SimplExprproof.SimplExpr_sepcomp_rel].
   eapply Tree.Forall2_reduce in T; eauto;
-    [|eapply (@link_program_sepcomp_rel Language_C Language_Clight id)]; simplify;
+    [|eapply (@link_program_sepcomp_rel Language.Language_C Language.Language_Clight id)]; simplify;
     [|apply SimplExpr_sig; auto].
   destruct T as [clightprog [Hclightprog Hclightsim]].
-  apply SimplExprproof_sepcomp.transl_program_correct in Hclightsim.
+  apply SimplExprproof.transl_program_correct in Hclightsim.
 
   (* Clight *)
   unfold transf_clight_program in TRANSF. clarify.
 
   eapply Tree.Forall2_reduce in T1; eauto;
-    [|eapply (transform_partial_program2_link_program Language_Clight Language_Clight)];
+    [|eapply (transform_partial_program2_link_program Language.Language_Clight Language.Language_Clight)];
     [|apply SimplLocals_sig].
   destruct T1 as [clight2prog [Hclight2prog Hclight2sim]].
   apply SimplLocalsproof.transf_program_correct in Hclight2sim.
 
   eapply Tree.Forall2_reduce in T0; eauto;
-    [|eapply (transform_partial_program2_link_program Language_Clight Language_Csharpminor)];
+    [|eapply (transform_partial_program2_link_program Language.Language_Clight Language.Language_Csharpminor)];
     [|apply Cshmgen_sig].
   destruct T0 as [csharpminorprog [Hsharpminorprog Hsharpminorsim]].
   apply Cshmgenproof.transl_program_correct in Hsharpminorsim.
 
   eapply Tree.Forall2_reduce in T; eauto;
-    [|eapply (transform_partial_program2_link_program Language_Csharpminor Language_Cminor)];
+    [|eapply (transform_partial_program2_link_program Language.Language_Csharpminor Language.Language_Cminor)];
     [|apply globfun_linkable_transf_partial_fundef];
     [|apply Cminorgen_sig].
   destruct T as [cminorprog [Hcminorprog Hcminorsim]].
@@ -272,24 +116,24 @@ Proof.
   assert (Hcheck_helpers: SelectLong.check_helpers (Genv.globalenv cminorprog) = OK tt).
   {
     exploit Tree.Forall_reduce; [| |eauto|].
-    - eapply Selectionproof_sepcomp.link_program_check_helpers.
+    - eapply Selectionproof.link_program_check_helpers.
     - clear -T0. revert p5 T0.
       induction p6; intros; inv T0; econstructor; eauto.
       monadInv Hpred. destruct x. auto.
     - auto.
   }
 
-  eapply Tree.Forall2_implies in T0; [|apply Selection_sepcomp_rel].
+  eapply Tree.Forall2_implies in T0; [|apply Selectionproof.Selection_sepcomp_rel].
   eapply Tree.Forall2_reduce in T0; eauto;
-    [|eapply (@link_program_sepcomp_rel Language_Cminor Language_CminorSel id)]; simplify;
+    [|eapply (@link_program_sepcomp_rel Language.Language_Cminor Language.Language_CminorSel id)]; simplify;
     [|eapply Selection_sig; eauto].
 
   destruct T0 as [cminorselprog [Hcminorselprog Hcminorselsim]].
-  apply Selectionproof_sepcomp.transl_program_correct in Hcminorselsim;
+  apply Selectionproof.transl_program_correct in Hcminorselsim;
     eauto using Selectionproof.check_helpers_correct.
 
   eapply Tree.Forall2_reduce in T; eauto;
-    [|eapply (transform_partial_program2_link_program Language_CminorSel Language_RTL)];
+    [|eapply (transform_partial_program2_link_program Language.Language_CminorSel Language.Language_RTL)];
     [|apply globfun_linkable_transf_partial_fundef];
     [|apply RTLgen_sig].
   destruct T as [rtlprog0 [Hrtlprog0 Hrtlsim0]].
@@ -304,41 +148,41 @@ Proof.
   destruct T19 as [rtlprog1 [Hrtlprog1 Hrtlsim1]]. subst.
   generalize (Tailcallproof.transf_program_correct rtlprog0) as Hrtlsim1. intro.
 
-  eapply Tree.Forall2_implies in T17; [|apply Inlining_sepcomp_rel].
-  eapply Tree.Forall2_reduce in T17; eauto; [|eapply (@link_program_sepcomp_rel Language_RTL Language_RTL id)]; simplify;
+  eapply Tree.Forall2_implies in T17; [|apply Inliningproof.Inlining_sepcomp_rel].
+  eapply Tree.Forall2_reduce in T17; eauto; [|eapply (@link_program_sepcomp_rel Language.Language_RTL Language.Language_RTL id)]; simplify;
     [|eapply Inlining_sig; eauto].
   destruct T17 as [rtlprog2 [Hrtlprog2 Hrtlsim2]].
-  apply Inliningproof_sepcomp.transf_program_correct in Hrtlsim2.
+  apply Inliningproof.transf_program_correct in Hrtlsim2.
 
   eapply Tree.Forall2_reduce in T15; eauto;
     [|eapply transform_program_link_program; auto].
   destruct T15 as [rtlprog3 [Hrtlprog3 Hrtlsim3]]. subst.
   generalize (Renumberproof.transf_program_correct rtlprog2) as Hrtlsim3. intro.
 
-  eapply Tree.Forall2_implies in T13; [|apply Constprop_sepcomp_rel].
-  eapply Tree.Forall2_reduce in T13; eauto; [|eapply (@link_program_sepcomp_rel Language_RTL Language_RTL id)]; simplify.
+  eapply Tree.Forall2_implies in T13; [|apply Constpropproof.Constprop_sepcomp_rel].
+  eapply Tree.Forall2_reduce in T13; eauto; [|eapply (@link_program_sepcomp_rel Language.Language_RTL Language.Language_RTL id)]; simplify.
   destruct T13 as [rtlprog4 [Hrtlprog4 Hrtlsim4]].
-  apply Constpropproof_sepcomp.transf_program_correct in Hrtlsim4.
+  apply Constpropproof.transf_program_correct in Hrtlsim4.
 
   eapply Tree.Forall2_reduce in T11; eauto;
     [|eapply transform_program_link_program; auto].
   destruct T11 as [rtlprog5 [Hrtlprog5 Hrtlsim5]]. subst.
   generalize (Renumberproof.transf_program_correct rtlprog4) as Hrtlsim5. intro.
 
-  eapply Tree.Forall2_implies in T9; [|apply CSE_sepcomp_rel].
-  eapply Tree.Forall2_reduce in T9; eauto; [|eapply (@link_program_sepcomp_rel Language_RTL Language_RTL id)]; simplify;
+  eapply Tree.Forall2_implies in T9; [|apply CSEproof.CSE_sepcomp_rel].
+  eapply Tree.Forall2_reduce in T9; eauto; [|eapply (@link_program_sepcomp_rel Language.Language_RTL Language.Language_RTL id)]; simplify;
     [|eapply CSE_sig; eauto].
   destruct T9 as [rtlprog6 [Hrtlprog6 Hrtlsim6]].
-  apply CSEproof_sepcomp.transf_program_correct in Hrtlsim6.
+  apply CSEproof.transf_program_correct in Hrtlsim6.
 
-  eapply Tree.Forall2_implies in T7; [|apply Deadcode_sepcomp_rel].
-  eapply Tree.Forall2_reduce in T7; eauto; [|eapply (@link_program_sepcomp_rel Language_RTL Language_RTL id)]; simplify;
+  eapply Tree.Forall2_implies in T7; [|apply Deadcodeproof.Deadcode_sepcomp_rel].
+  eapply Tree.Forall2_reduce in T7; eauto; [|eapply (@link_program_sepcomp_rel Language.Language_RTL Language.Language_RTL id)]; simplify;
     [|eapply Deadcode_sig; eauto].
   destruct T7 as [rtlprog7 [Hrtlprog7 Hrtlsim7]].
-  apply Deadcodeproof_sepcomp.transf_program_correct in Hrtlsim7.
+  apply Deadcodeproof.transf_program_correct in Hrtlsim7.
 
   eapply Tree.Forall2_reduce in T5; eauto;
-    [|eapply (transform_partial_program2_link_program Language_RTL Language_LTL)];
+    [|eapply (transform_partial_program2_link_program Language.Language_RTL Language.Language_LTL)];
     [|apply globfun_linkable_transf_partial_fundef];
     [|apply Allocation_sig].
   destruct T5 as [ltlprog0 [Hltlprog0 Hltlsim0]].
@@ -350,7 +194,7 @@ Proof.
   generalize (Tunnelingproof.transf_program_correct ltlprog0) as Hltlsim1. intro.
 
   eapply Tree.Forall2_reduce in T2; eauto;
-    [|eapply (transform_partial_program2_link_program Language_LTL Language_Linear)];
+    [|eapply (transform_partial_program2_link_program Language.Language_LTL Language.Language_Linear)];
     [|apply globfun_linkable_transf_partial_fundef];
     [|apply Linearize_sig].
   destruct T2 as [linearprog0 [Hlinearprog0 Hlinearsim0]].
@@ -362,7 +206,7 @@ Proof.
   generalize (CleanupLabelsproof.transf_program_correct linearprog0) as Hlinearsim1. intro.
 
   eapply Tree.Forall2_reduce in T0; eauto;
-    [|eapply (transform_partial_program2_link_program Language_Linear Language_Mach)];
+    [|eapply (transform_partial_program2_link_program Language.Language_Linear Language.Language_Mach)];
     [|apply globfun_linkable_transf_partial_fundef];
     [|apply Stacking_sig].
   destruct T0 as [machprog [Hmachprog Hmachsim]].
@@ -370,7 +214,7 @@ Proof.
     [|eexact Asmgenproof.return_address_exists; eassumption].
 
   eapply Tree.Forall2_reduce in TRANSF; eauto;
-    [|eapply (transform_partial_program2_link_program Language_Mach Language_Asm)];
+    [|eapply (transform_partial_program2_link_program Language.Language_Mach Language.Language_Asm)];
     [|apply globfun_linkable_transf_partial_fundef];
     [|apply Asmgen_sig].
   destruct TRANSF as [asmprog [Hasmprog Hasmsim]].
@@ -383,11 +227,11 @@ Qed.
 
 Lemma linker_correct_determinate
         ctree asmtree cprog
-        (CLINK: Tree.reduce (link_program Language_C) ctree = Some cprog)
+        (CLINK: Tree.reduce (link_program Language.Language_C) ctree = Some cprog)
         (TRANSF: Tree.Forall2 (fun c a => transf_c_program c = OK a) ctree asmtree):
   exists (asmprog:Asm.program)
     (_:backward_simulation (atomic (Cstrategy.semantics cprog)) (Asm.semantics asmprog)),
-    Tree.reduce (link_program Language_Asm) asmtree = Some asmprog.
+    Tree.reduce (link_program Language.Language_Asm) asmtree = Some asmprog.
 Proof.
   exploit linker_correct_determinate_forward; eauto.
   intros [asmprog [Hsim Hasmprog]]. exists asmprog.
@@ -400,11 +244,11 @@ Qed.
 
 Theorem linker_correct
         ctree asmtree cprog
-        (CLINK: Tree.reduce (link_program Language_C) ctree = Some cprog)
+        (CLINK: Tree.reduce (link_program Language.Language_C) ctree = Some cprog)
         (TRANSF: Tree.Forall2 (fun c a => transf_c_program c = OK a) ctree asmtree):
   exists (asmprog:Asm.program)
     (_:backward_simulation (Csem.semantics cprog) (Asm.semantics asmprog)),
-    Tree.reduce (link_program Language_Asm) asmtree = Some asmprog.
+    Tree.reduce (link_program Language.Language_Asm) asmtree = Some asmprog.
 Proof.
   exploit linker_correct_determinate; eauto.
   intros [asmprog [Hsim Hasmprog]]. exists asmprog.
